updated SWAP decomposition

VOQC/GreedyLayout.v
@@ -10,29 +10,20 @@ Module FSet := FSetAVL.Make(Coq.Structures.OrderedTypeEx.Nat_as_OT).
 Module FSetFacts := FSetFacts.Facts FSet.
 Module FSetProps := FSetProperties.Properties FSet.
 
+Local Open Scope nat_scope.
+
 (** Choose an initial logical->physical qubit mapping (i.e., layout) for a
     program that puts qubits close together on the architecture if they are 
     used together in a two-qubit gate. *)
 
 (** Choose an unused qubit based on the given preferences. *)
-Fixpoint get_default (prefs : list nat) (alloc : FSet.t) :=
+Fixpoint get_fresh_qubit (prefs : list nat) (alloc : FSet.t) :=
   match prefs with
-  | [] => O (* unreachable unless all qubits are allocated *)
+  | [] => O (* unreachable, per conditions in the proof *)
   | p :: prefs => 
       if FSet.mem p alloc 
-      then get_default prefs alloc 
+      then get_fresh_qubit prefs alloc 
       else p
-  end.
-
-(** Choose an unused qubit given a list of cadidates (ordered best -> worst)
-    and a set of used qubits. *)
-Fixpoint get_unused (cands : list nat) (prefs : list nat) (alloc : FSet.t) :=
-  match cands with 
-  | [] => get_default prefs alloc
-  | c :: cands => 
-      if FSet.mem c alloc 
-      then get_unused cands prefs alloc 
-      else c
   end.
 
 (** Build a layout based on the structure of the input program.
@@ -45,54 +36,499 @@ Fixpoint get_unused (cands : list nat) (prefs : list nat) (alloc : FSet.t) :=
    in the returned layout. Note that the layout may change during mapping 
    (due to inserted swaps) so this strategy will not always choose the best 
    placement. *)
-Fixpoint build_layout {U dim} (l : gate_list (Map_Unitary U) dim) (alloc : FSet.t) (lay : layout) (get_nearby : nat -> list nat) (q_ordering : list nat) : FSet.t * layout:=
+Fixpoint build_layout {U dim} (l : gate_list (Map_Unitary U) dim) (alloc : FSet.t) (lay : layout) (q_ordering : option nat -> list nat) : FSet.t * layout:=
   match l with
   | [] => (alloc, lay)
   | App2 UMap_CNOT m n :: t => 
-      match find_phys lay m, find_phys lay m with
-      | Some _, Some _ => build_layout t alloc lay get_nearby q_ordering
+      match find_phys lay m, find_phys lay n with
+      | Some _, Some _ => build_layout t alloc lay q_ordering
       | Some m_phys, None =>
-          let n_phys := get_unused (get_nearby m_phys) q_ordering alloc in
+          let n_phys := get_fresh_qubit (q_ordering (Some m_phys)) alloc in
           let alloc' := FSet.add n_phys alloc in
           let lay' := add lay n n_phys in
-          build_layout t alloc' lay' get_nearby q_ordering
+          build_layout t alloc' lay' q_ordering
       | None, Some n_phys =>
-          let m_phys := get_unused (get_nearby n_phys) q_ordering alloc in
+          let m_phys := get_fresh_qubit (q_ordering (Some n_phys)) alloc in
           let alloc' := FSet.add m_phys alloc in
           let lay' := add lay m m_phys in
-          build_layout t alloc' lay' get_nearby q_ordering
+          build_layout t alloc' lay' q_ordering
       | None, None =>
-          let m_phys := get_default q_ordering alloc in
-          let n_phys := get_unused (get_nearby m_phys) q_ordering alloc in
+          let m_phys := get_fresh_qubit (q_ordering None) alloc in
+          let n_phys := get_fresh_qubit (q_ordering (Some m_phys)) alloc in
           let alloc' := FSet.add n_phys (FSet.add m_phys alloc) in
           let lay' := add (add lay m m_phys) n n_phys in
-          build_layout t alloc' lay' get_nearby q_ordering
+          build_layout t alloc' lay' q_ordering
       end
-  | _ :: t => build_layout t alloc lay get_nearby q_ordering
+  | _ :: t => build_layout t alloc lay q_ordering
   end.
 
 (** Choose a physical qubit for any unallocated logical qubits. n is the number
     of physical qubits available. *)
-Fixpoint extend_layout (n : nat) (alloc : FSet.t) (lay : layout) (q_ordering : list nat)  :=
+Fixpoint extend_layout (n : nat) (alloc : FSet.t) (lay : layout) (q_ordering : option nat -> list nat)  :=
   match n with
   | O => lay
   | S n' => 
       match find_phys lay n' with 
       | Some _ => extend_layout n' alloc lay q_ordering
-      | None => let m := get_default q_ordering alloc in
+      | None => let m := get_fresh_qubit (q_ordering None) alloc in
                extend_layout n' (FSet.add m alloc) (add lay n' m) q_ordering
       end
-  end. 
+  end.
 
 (** dim is the number of qubits used in the program l and n is the number of
    qubits available on the machine *)
-Definition greedy_layout {U dim} (l : gate_list (Map_Unitary U) dim) (n : nat) (get_nearby : nat -> list nat) (q_ordering : list nat) : layout :=
-  let (alloc, lay) := build_layout l FSet.empty empty get_nearby q_ordering in
+Definition greedy_layout {U dim} (l : gate_list (Map_Unitary U) dim) (n : nat) (q_ordering : option nat -> list nat) : layout :=
+  let (alloc, lay) := build_layout l FSet.empty empty q_ordering in
   extend_layout n alloc lay q_ordering.
 
-Lemma greedy_layout_bijective : forall U dim (l : gate_list (Map_Unitary U) dim) n get_nearby q_ordering,
-  (* some preconditions ... *)
-  layout_bijective n (greedy_layout l n get_nearby q_ordering).
+(** Proofs *)
+
+Lemma get_fresh_qubit_lt : forall prefs alloc n,
+  (forall x, In x prefs -> x < n) -> 
+  (exists x, In x prefs /\ ~ FSet.In x alloc) ->
+  get_fresh_qubit prefs alloc < n.
 Proof.
-(* TODO *)
+  intros prefs alloc n Hn H.
+  induction prefs; simpl.
+  destruct H as [? [H ?]].
+  inversion H.
+  destruct H as [x [Hx1 Hx2]].
+  bdestruct (x =? a). subst.
+  destruct (FSet.mem a alloc) eqn:fmem.
+  apply FSetFacts.mem_iff in fmem.
+  contradiction.
+  apply Hn. left. auto.
+  destruct (FSet.mem a alloc).
+  apply IHprefs.
+  intros. apply Hn. right. auto.
+  exists x. split; auto. 
+  inversion Hx1. subst. contradiction. auto.
+  apply Hn. left. auto.
+Qed.
+
+Lemma get_fresh_qubit_not_In_alloc : forall prefs alloc,
+  (exists x, In x prefs /\ ~ FSet.In x alloc) ->
+  ~ FSet.In (get_fresh_qubit prefs alloc) alloc.
+Proof.
+  intros prefs alloc H.
+  induction prefs; simpl.
+  destruct H as [? [H ?]].
+  inversion H.
+  destruct H as [x [Hx1 Hx2]].
+  bdestruct (x =? a). subst.
+  destruct (FSet.mem a alloc) eqn:fmem.
+  apply FSetFacts.mem_iff in fmem.
+  contradiction. auto.
+  destruct (FSet.mem a alloc) eqn:fmem.
+  apply IHprefs.
+  exists x. split; auto. 
+  inversion Hx1. subst. contradiction. auto.
+  apply FSetFacts.not_mem_iff.
+  assumption.
+Qed.
+
+Definition alloc_records_allocated_phys_qubits lay alloc :=
+  forall p, FSet.In p alloc <-> exists l, find_phys lay l = Some p.
+
+Definition find_log_bounded lay n := 
+ forall p l, find_log lay p = Some l -> l < n.
+
+Definition find_phys_bounded lay n := 
+ forall l p, find_phys lay l = Some p -> p < n.
+
+Lemma alloc_records_allocated_phys_qubits_add : forall lay alloc l p,
+  find_phys lay l = None ->
+  alloc_records_allocated_phys_qubits lay alloc ->
+  alloc_records_allocated_phys_qubits (add lay l p) (FSet.add p alloc).
+Proof.
+  intros lay alloc l p Hl H.
+  unfold alloc_records_allocated_phys_qubits in *.
+  intro p0.
+  bdestruct (p0 =? p). subst.
+  split; intro.
+  exists l.
+  apply find_phys_add_eq.
+  apply FSet.add_1; auto.
+  split; intro.
+  apply FSet.add_3 in H1; auto.
+  apply H in H1.
+  destruct H1 as [l0 H1].
+  exists l0.
+  rewrite find_phys_add_neq; auto.
+  intro contra. subst.
+  rewrite Hl in H1.
+  inversion H1.
+  destruct H1 as [l0 H1].
+  apply FSet.add_2.
+  apply H.
+  exists l0.
+  rewrite find_phys_add_neq in H1; auto.
+  intro contra. subst.
+  rewrite find_phys_add_eq in H1.
+  inversion H1; subst.
+  contradiction.
+Qed.
+
+Definition find_log_bounded_add : forall lay n l p,
+  find_log_bounded lay n -> l < n -> find_log_bounded (add lay l p) n.
+Proof.
+  intros lay n l p H Hl.
+  unfold find_log_bounded in *.
+  intros p0 l0 Hadd.
+  bdestruct (p =? p0); subst.
+  rewrite find_log_add_eq in Hadd.
+  inversion Hadd; subst. auto.
+  rewrite find_log_add_neq in Hadd by auto.
+  apply H in Hadd. auto.
+Qed.
+
+Definition find_phys_bounded_add : forall lay n l p,
+  find_phys_bounded lay n -> p < n -> find_phys_bounded (add lay l p) n.
+Proof.
+  intros lay n l p H Hp.
+  unfold find_phys_bounded in *.
+  intros l0 p0 Hadd.
+  bdestruct (l =? l0); subst.
+  rewrite find_phys_add_eq in Hadd.
+  inversion Hadd; subst. auto.
+  rewrite find_phys_add_neq in Hadd by auto.
+  apply H in Hadd. auto.
+Qed.
+
+(* TODO: move to CG *)
+Definition valid_q_ordering (q_ordering : option nat -> list nat) n :=
+  forall o x, x < n <-> List.In x (q_ordering o).
+
+(* Easy definition that satisfies the spec *)
+Fixpoint list_nats n := match n with O => [] | S n' => n' :: list_nats n' end.
+
+Lemma list_nats_is_valid_q_ordering : forall n, valid_q_ordering (fun _ => list_nats n) n.
+Proof.
+  intros n o x.
+  induction n; simpl.
+  lia.
+  bdestruct (x =? n).
+  subst.
+  split; intro H; auto.
+  split; intro H0.
+  right. apply IHn. lia.
+  destruct H0 as [H0 | H0]; subst; try contradiction.
+  apply IHn in H0. lia.
+Qed.
+
+Lemma find_phys_None_implies_alloc_incomplete : forall lay alloc q_ord n o,
+  valid_q_ordering q_ord n ->
+  well_formed lay ->
+  alloc_records_allocated_phys_qubits lay alloc ->
+  find_log_bounded lay n ->
+  find_phys_bounded lay n ->
+  (exists x, x < n /\ find_phys lay x = None) ->
+  exists x : FSet.elt, In x (q_ord o) /\ ~ FSet.In x alloc.
+Proof.
+  intros lay alloc q_ord n o Hqor WF Halloc Hlog Hphys [x [Hx1 Hx2]].
+
+
+(* stuck -- we probably need some kind of counting argument *)
+
 Admitted.
+
+Lemma build_layout_well_formed : forall U dim (l : gate_list (Map_Unitary U) dim) alloc lay q_ordering lay' alloc',
+  well_formed lay ->
+  uc_well_typed_l l ->
+  alloc_records_allocated_phys_qubits lay alloc ->
+  find_log_bounded lay dim ->
+  find_phys_bounded lay dim ->
+  valid_q_ordering q_ordering dim ->
+  build_layout l alloc lay q_ordering = (alloc', lay') ->
+  well_formed lay' /\
+  alloc_records_allocated_phys_qubits lay' alloc' /\
+  find_log_bounded lay' dim /\
+  find_phys_bounded lay' dim.
+Proof.
+  intros U dim l alloc lay q_ordering lay' alloc' WF WT Halloc Hlog Hphys Hqor H.
+  gen alloc lay.
+  induction l; intros alloc lay WF Halloc Hlog Hphys H.
+  simpl in *.
+  inversion H; subst.
+  auto.
+  simpl in H.
+  destruct a; dependent destruction m; inversion WT; subst; try apply IHl in H; auto.
+  destruct (find_phys lay n) eqn:fpn; destruct (find_phys lay n0) eqn:fpn0.
+  - apply IHl in H; auto.
+  - remember (get_fresh_qubit (q_ordering (Some n1)) alloc) as x.
+    apply IHl in H; auto; clear IHl.
+    apply add_well_formed; auto.
+    intros [contra | contra].
+    apply Halloc in contra.
+    contradict contra.
+    subst. apply get_fresh_qubit_not_In_alloc.
+    eapply find_phys_None_implies_alloc_incomplete.
+    apply Hqor. apply WF. apply Halloc. apply Hlog. apply Hphys.
+    exists n0. split; auto.
+    destruct contra as [p contra].
+    apply WF in contra.
+    rewrite fpn0 in contra.
+    inversion contra.
+    apply alloc_records_allocated_phys_qubits_add; auto.
+    apply find_log_bounded_add; auto.
+    apply find_phys_bounded_add; auto.
+    subst. apply get_fresh_qubit_lt.
+    intros. apply Hqor in H0. auto.
+    eapply find_phys_None_implies_alloc_incomplete.
+    apply Hqor. apply WF. apply Halloc. apply Hlog. apply Hphys.
+    exists n0. split; auto.
+  - remember (get_fresh_qubit (q_ordering (Some n)) alloc) as x.
+    apply IHl in H; auto; clear IHl.
+    apply add_well_formed; auto.
+    intros [contra | contra].
+    apply Halloc in contra.
+    contradict contra.
+    subst. apply get_fresh_qubit_not_In_alloc.
+    eapply find_phys_None_implies_alloc_incomplete.
+    apply Hqor. apply WF. apply Halloc. apply Hlog. apply Hphys.
+    exists n. split; auto.
+    destruct contra as [p contra].
+    apply WF in contra.
+    rewrite fpn in contra.
+    inversion contra.
+    apply alloc_records_allocated_phys_qubits_add; auto.
+    apply find_log_bounded_add; auto.
+    apply find_phys_bounded_add; auto.
+    subst. apply get_fresh_qubit_lt.
+    intros. apply Hqor in H0. auto.
+    eapply find_phys_None_implies_alloc_incomplete.
+    apply Hqor. apply WF. apply Halloc. apply Hlog. apply Hphys.
+    exists n. split; auto.
+  - remember (get_fresh_qubit (q_ordering None) alloc) as x.
+    remember (get_fresh_qubit (q_ordering (Some x)) (FSet.add x alloc)) as y.
+    apply IHl in H; auto; clear IHl.
+    apply add_well_formed; auto.
+    apply add_well_formed; auto.
+    intros [contra | contra].
+    apply Halloc in contra.
+    contradict contra.
+    subst. apply get_fresh_qubit_not_In_alloc.
+    eapply find_phys_None_implies_alloc_incomplete.
+    apply Hqor. apply WF. apply Halloc. apply Hlog. apply Hphys.
+    exists n. split; auto.
+    destruct contra as [p contra].
+    apply WF in contra.
+    rewrite fpn in contra.
+    inversion contra. 
+    apply not_In_add; auto.
+     admit. (* y <> x ; y is not in (FSet.add x alloc) *)
+    intros [contra | contra].
+    apply Halloc in contra.
+    contradict contra.
+    subst. apply get_fresh_qubit_not_In_alloc.
+    eapply find_phys_None_implies_alloc_incomplete.
+    apply Hqor. apply WF. apply Halloc. apply Hlog. apply Hphys.
+    exists n. split; auto.
+    destruct contra as [p contra].
+    apply WF in contra.
+    rewrite fpn0 in contra.
+    inversion contra.
+    apply alloc_records_allocated_phys_qubits_add; auto.
+    rewrite find_phys_add_neq; auto.
+    apply alloc_records_allocated_phys_qubits_add; auto.
+    apply find_log_bounded_add; auto.
+    apply find_log_bounded_add; auto.
+    apply find_phys_bounded_add; auto.
+    apply find_phys_bounded_add; auto.
+    subst. apply get_fresh_qubit_lt.
+    intros. apply Hqor in H0. auto.
+    eapply find_phys_None_implies_alloc_incomplete.
+    apply Hqor. apply WF. apply Halloc. apply Hlog. apply Hphys.
+    exists n. split; auto.
+    subst. apply get_fresh_qubit_lt.
+    intros. apply Hqor in H0. auto.
+    eapply find_phys_None_implies_alloc_incomplete.
+    apply Hqor. apply WF. apply Halloc. apply Hlog. apply Hphys.
+    exists n. split; auto.
+Admitted.
+
+Lemma find_log_extend_layout1 : forall n alloc lay q_ordering p l,
+  alloc_records_allocated_phys_qubits lay alloc ->
+  find_log lay p = Some l ->
+  find_log (extend_layout n alloc lay q_ordering) p = Some l.
+Proof.
+  intros n alloc lay q_ordering p l.
+  gen alloc lay.
+  induction n; intros alloc lay H1 H2; simpl; auto.
+  destruct (find_phys lay n) eqn:fp.
+  auto.
+  apply IHn.
+  apply alloc_records_allocated_phys_qubits_add; auto.
+  rewrite find_log_add_neq; auto.
+  (* "get_default q_ordering alloc" is not in alloc, but p is *)
+Admitted.
+
+Lemma find_log_extend_layout2 : forall m n alloc lay q_ordering p,
+  (p < n)%nat ->
+  well_formed lay ->
+  alloc_records_allocated_phys_qubits lay alloc ->
+  find_log lay p = None ->
+  exists l, find_log (extend_layout n alloc lay q_ordering) p = Some l /\ (l < m)%nat.
+Proof.
+  intros m n alloc lay q_ordering p Hp.
+  gen alloc lay.
+  induction n; intros alloc lay H1 H2 H3; simpl; auto.
+lia.
+
+(*
+bdestruct (p =? n).
+subst. clear IHn.
+
+destruct (find_phys lay n) eqn:fp.
+
+  exists (get_default q_ordering alloc).
+  split.
+  erewrite find_phys_extend_layout1.
+  reflexivity.
+  apply alloc_records_allocated_phys_qubits_add; auto.
+  apply find_phys_add_eq.
+
+
+admit.
+
+
+destruct (find_phys lay n) eqn:fp.
+
+apply IHn; auto. lia.
+
+apply IHn. lia.
+  apply alloc_records_allocated_phys_qubits_add; auto.
+  rewrite find_log_add_neq; auto.
+*)
+
+ Admitted.
+
+Lemma find_phys_extend_layout1 : forall n alloc lay q_ordering l p,
+  alloc_records_allocated_phys_qubits lay alloc ->
+  find_phys lay l = Some p ->
+  find_phys (extend_layout n alloc lay q_ordering) l = Some p.
+Proof.
+  intros n alloc lay q_ordering l p.
+  gen alloc lay.
+  induction n; intros alloc lay H1 H2; simpl; auto.
+  destruct (find_phys lay n) eqn:fp.
+  auto.
+  apply IHn.
+  apply alloc_records_allocated_phys_qubits_add; auto.
+  rewrite find_phys_add_neq; auto.
+  intro contra. subst.
+  rewrite H2 in fp. inversion fp.
+Qed.
+
+Lemma find_phys_extend_layout2 : forall m n alloc lay q_ordering l,
+  (l < n)%nat ->
+  well_formed lay ->
+  alloc_records_allocated_phys_qubits lay alloc ->
+  valid_q_ordering q_ordering m ->
+  find_phys lay l = None ->
+  exists p, find_phys (extend_layout n alloc lay q_ordering) l = Some p /\ (p < m)%nat.
+Proof.
+  intros m n alloc lay q_ordering l Hl ? ? Hqor.
+  gen alloc lay.
+  induction n; intros alloc lay WF Halloc H; simpl; auto.
+  lia.
+  bdestruct (l =? n).
+  subst. clear IHn.
+  rewrite H.
+  exists (get_fresh_qubit (q_ordering None) alloc).
+  split.
+  erewrite find_phys_extend_layout1.
+  reflexivity.
+  apply alloc_records_allocated_phys_qubits_add; auto.
+  apply find_phys_add_eq.
+  apply get_fresh_qubit_lt.
+  intros. apply Hqor in H0. auto.
+  eapply find_phys_None_implies_alloc_incomplete.
+  apply Hqor. apply WF. apply Halloc. (*apply Hlog. apply Hphys.
+  exists n. split; auto.
+  admit. (*  (get_default q_ordering alloc < m)%nat *)
+  destruct (find_phys lay n) eqn:fp.
+  apply IHn; auto. lia.
+  apply IHn. lia.
+  apply alloc_records_allocated_phys_qubits_add; auto.
+  rewrite find_phys_add_neq; auto.*)
+Admitted.
+
+Lemma extend_layout_well_formed : forall n alloc lay q_ordering,
+  well_formed lay ->
+  alloc_records_allocated_phys_qubits lay alloc ->
+  well_formed (extend_layout n alloc lay q_ordering).
+Proof.
+  intros n alloc lay q_ordering.
+  gen alloc lay.
+  induction n; intros alloc lay H1 H2; simpl; auto.
+  destruct (find_phys lay n) eqn:fp.
+  apply IHn; auto.
+  apply IHn.
+  apply add_well_formed; auto.
+  apply Classical_Prop.and_not_or.
+  split.
+  intro contra.
+  apply H2 in contra.
+  assert (~ (FSet.In (get_fresh_qubit (q_ordering None) alloc) alloc)).
+  admit.
+  contradiction.
+  intros [p contra].
+  apply H1 in contra.
+  rewrite fp in contra.
+  inversion contra.
+  apply alloc_records_allocated_phys_qubits_add; auto.
+Admitted.
+
+Lemma extend_layout_bijective : forall n alloc lay q_ordering,
+  well_formed lay ->
+  alloc_records_allocated_phys_qubits lay alloc ->
+  find_log_bounded lay n ->
+  find_phys_bounded lay n ->
+  valid_q_ordering q_ordering n ->
+  layout_bijective n (extend_layout n alloc lay q_ordering).
+Proof.
+  intros n alloc lay q_ordering WF H1 H2 H3 H4.
+  split; [|split].
+  - apply extend_layout_well_formed; auto.
+  - intros l Hl.
+    destruct (find_phys lay l) eqn:fp.
+    exists n0.
+    split.
+    apply find_phys_extend_layout1; auto.
+    apply H3 in fp. auto.
+    apply find_phys_extend_layout2; auto.
+  - intros p Hp.
+    destruct (find_log lay p) eqn:fl.
+    exists n0.
+    split.
+    apply find_log_extend_layout1; auto.
+    apply H2 in fl. auto.
+    apply find_log_extend_layout2; auto.
+Qed.
+
+(** dim is the number of qubits used in the program l and n is the number of
+   qubits available on the machine *)
+Lemma greedy_layout_bijective : forall U dim (l : gate_list (Map_Unitary U) dim) q_ordering,
+  uc_well_typed_l l ->
+  valid_q_ordering q_ordering dim ->
+  layout_bijective dim (greedy_layout l dim q_ordering).
+Proof.
+  intros U dim l qubit_ordering WT Hqor.
+  unfold greedy_layout.
+  destruct (build_layout l FSet.empty empty qubit_ordering) eqn:bl.
+  apply build_layout_well_formed with (dim:=dim) in bl as [? [? [? ?]]]; auto.
+  apply extend_layout_bijective; auto.
+  apply empty_well_formed.
+  split; intro H.
+  apply FSetFacts.empty_iff in H. easy.
+  destruct H as [? H].
+  rewrite find_phys_empty in H.
+  inversion H.
+  intros ? ? H.
+  rewrite find_log_empty in H.
+  inversion H.
+  intros ? ? H.
+  rewrite find_phys_empty in H.
+  inversion H.
+Qed.
