VOQC/MappingConstraints.v
@@ -41,6 +41,75 @@ Proof.
   constructor; auto.
 Qed.
 
+Lemma respects_constraints_undirected_app_split : forall {U dim} (l1 l2 : gate_list U dim) is_in_graph,
+  respects_constraints_undirected is_in_graph (l1 ++ l2) ->
+  respects_constraints_undirected is_in_graph l2 /\
+  respects_constraints_undirected is_in_graph l1.
+Proof.
+  intros U dim l1 l2 is_in_graph H.
+  split.
+  - induction l1.
+    simpl in H.
+    assumption.
+    rewrite <- app_comm_cons in H.
+    destruct a; remember (l1 ++ l2) as l; inversion H; subst;
+      try (apply IHl1 in H2); auto.
+  - induction l1.
+    constructor.
+    rewrite <- app_comm_cons in H;   
+      destruct a; remember (l1 ++ l2) as l; inversion H; subst.
+    constructor; auto.
+    constructor; auto.
+Qed.
+
+Lemma rev_respects_constraints_undirected:
+  forall {U dim} (l : gate_list U dim) (is_in_graph : nat -> nat -> bool),
+    respects_constraints_undirected is_in_graph l ->
+    respects_constraints_undirected is_in_graph (rev l).
+Proof.
+  intros.
+  induction l; simpl; auto.
+  destruct a; inversion H; subst.
+  apply respects_constraints_undirected_app; auto.
+  constructor. constructor.
+  apply respects_constraints_undirected_app; auto.
+  constructor. auto. constructor.
+Qed. 
+
+Lemma rev_append_respects_constraints_undirected:
+  forall {U dim} (l1 l2 : gate_list U dim) (is_in_graph : nat -> nat -> bool),
+    respects_constraints_undirected is_in_graph l1 ->
+    respects_constraints_undirected is_in_graph l2 ->
+    respects_constraints_undirected is_in_graph (rev_append l1 l2).
+Proof.
+  intros.
+  rewrite rev_append_rev.
+  apply respects_constraints_undirected_app.
+  apply rev_respects_constraints_undirected.
+  assumption.
+  assumption.
+Qed.
+
+Lemma next_two_qubit_gate_respects_constraints_undirected:
+  forall {U dim} (l l1 l2: gate_list U dim) g (q q1 q2 : nat) (is_in_graph : nat -> nat -> bool),
+  respects_constraints_undirected is_in_graph l ->
+  next_two_qubit_gate l q = Some (l1, g, q1, q2, l2) ->
+  respects_constraints_undirected is_in_graph l1
+    /\ respects_constraints_undirected is_in_graph l2 /\ 
+      (is_in_graph q1 q2 = true \/ is_in_graph q2 q1 = true).
+Proof.
+  intros.
+  apply ntqg_preserves_structure in H0. 
+  rewrite H0 in H. 
+  eapply respects_constraints_undirected_app_split in H.
+  destruct H as [rcdapp rcdl1].
+  eapply respects_constraints_undirected_app_split in rcdapp.
+  destruct rcdapp as [rcdl2 rcdapp2].
+  repeat split; auto.
+  inversion rcdapp2; subst.
+  assumption.
+Qed.
+
 Lemma respects_constraints_directed_app : forall {U dim} (l1 l2 : gate_list U dim) is_in_graph cnot,
   respects_constraints_directed is_in_graph cnot l1 ->
   respects_constraints_directed is_in_graph cnot l2 ->
